providers/evercrypt/EverCrypt.Hash.fsti
@@ -198,7 +198,7 @@ val frame_invariant: #a:alg -> l:M.loc -> s:state a -> h0:HS.mem -> h1:HS.mem ->
   (requires (
     invariant s h0 /\
     M.loc_disjoint l (footprint s h0) /\
-    M.modifies_inert l h0 h1))
+    M.modifies l h0 h1))
   (ensures (
     invariant s h1 /\
     repr s h0 == repr s h1))
@@ -211,7 +211,7 @@ let frame_invariant_implies_footprint_preservation
   (requires (
     invariant s h0 /\
     M.loc_disjoint l (footprint s h0) /\
-    M.modifies_inert l h0 h1))
+    M.modifies l h0 h1))
   (ensures (
     footprint s h1 == footprint s h0))
 =
